theories/AlmostStlc/SemanticsFactsSeq.v
@@ -1,6 +1,9 @@
 Require Export TypedVar.
 Require Export SyntaxSeq.
 Require Export SmallStepSeq.
+Require Export DenotationFacts.
+Require Export DenotationSeq.
+Import List.ListNotations.
 Open Scope list_scope.
 From Equations Require Import Equations Signature.
 Require Import Coq.Program.Equality.
@@ -8,8 +11,9 @@ Require Import ExtLib.Structures.Monad.
 Import MonadNotation.
 Local Open Scope monad_scope.
 
+Notation call_syn := SmallStepSeq.call.
 (* bottoms out in exposed contexts *)
-Inductive covered_in {t2 MR2} (ca : call t2 MR2) 
+Inductive covered_in {t2 MR2} (ca : call_syn t2 MR2) 
   : forall t1 MR1 (b : bool) 
           (E : eval_context t1 MR1 (inr ca) b),  Prop :=
   (* need three base cases, one for each handler style context *)
@@ -46,14 +50,14 @@ Inductive covered_in {t2 MR2} (ca : call t2 MR2)
 Arguments covered_in {_ _} (_) {_ _ _}.
 
 (* need to be a bit more general, allow for an MR1 but force b = false *)
-Lemma covered_in_intro t1 t2 MR1 MR2 (ca : call t2 MR2) (E : eval_context t1 MR1 (inr ca) false) : 
+Lemma covered_in_intro t1 t2 MR1 MR2 (ca : call_syn t2 MR2) (E : eval_context t1 MR1 (inr ca) false) : 
   covered_in ca E.
 Proof.
   dependent induction E; try (destruct b; constructor; auto).
   constructor. apply IHE; auto.
 Qed.
 
-Lemma covered_in_step t1 t2 MR1 MR2 b (ca : call t2 MR2) (E : eval_context t1 MR1 (inr ca) b) :
+Lemma covered_in_step t1 t2 MR1 MR2 b (ca : call_syn t2 MR2) (E : eval_context t1 MR1 (inr ca) b) :
   covered_in ca E -> exists c, step_eval_context b (inr ca) E = Some c.
 Proof.
   intros H. dependent induction H; simp step_eval_context.
@@ -73,7 +77,7 @@ Qed.
    if ca is covered 
 *)
 
-Lemma progress_boxed_eval_context (t1 t2 : vtype) b (MR : mfix_ctx) (r : bredex t2 MR + call t2 MR) (E : eval_context t1 nil r b) : 
+Lemma progress_boxed_eval_context (t1 t2 : vtype) b (MR : mfix_ctx) (r : bredex t2 MR + call_syn t2 MR) (E : eval_context t1 nil r b) : 
   exists c, step_eval_context b r E = Some c.
 Proof.
   destruct r.
@@ -88,58 +92,178 @@ Qed.
 Theorem progress_step (t : vtype) (c : comp t nil nil) :
   (exists c', step c = inl (Some c')) \/ (exists v, step c = inr v).
 Proof.
-  unfold step. destruct (observe c); eauto.
+  unfold step. destruct (SmallStepSeq.observe c); eauto.
   destruct b. left.
   specialize progress_boxed_eval_context with (E := E) as [c' Hc'].
   rewrite Hc'. eexists. reflexivity.
 Qed.
-
 (*
-  dependent induction E; destruct r; try (simp step_eval_context; eexists; eauto; fail).
-  - inversion c. inversion xR. 
-  - simp step_eval_context.
-    specialize (IHE E eq_refl JMeq_refl). destruct IHE as [c' Hc].
-    rewrite Hc. cbn. eexists. eauto.
-  - simp step_eval_context.
-    assert (MR1 = R :: nil).
-    {
-      destruct xR; simp remove in x0; subst; auto.
-      discriminate.
-    }
-    subst. clear x0. 
-
-    dependent destruction x.
-    assert (xR = VarZ).
-    { clear - xR. dependent destruction xR. auto. inversion xR. }
-    subst. simp remove in x0.
-    apply JMeq_eq in x. subst.
-    clear x0. 
-    destruct b.
-    + specialize step_eval_context_equation_4 with (bodies := bodies) (E := E) 
-        (xR := VarZ) as Heq. destruct (normalize_eval_context c E).
-      destruct x. 
-      match goal with Heq : _ = ret ?x |- _ => set x as c0 end.
-      exists c0. auto.
-    + eexists. specialize step_eval_context_equation_5 with (bodies := bodies) (E := E) 
-        (xR := VarZ) as Heq. 
-      (* need a stronger inductive hypothesis, maybe a logical relation
-       should encode the idea of a handled call_frame
-       *)
-      admit.
-  - assert (MR1 = nil).
-    { clear - Hperm. dependent induction Hperm. auto. eapply IHHperm1. auto. }
-    subst. specialize (IHE E eq_refl JMeq_refl).
-    destruct IHE as [c0 Hc0]. destruct b. simp step_eval_context; subst; cbn.
-    + destruct (normalize_eval_context c E). destruct x. eexists. reflexivity.
-    + simp step_eval_context. rewrite Hc0. cbn. eexists. eauto.
-  - (* stop here for now, tomorrow finish this progress lemma, and use it 
-       to prove the full progress theorem (show be trivial),
-       also see if you can write the denotation function,
-
-       and maybe get started on lemmas that substitution is like denoting 
-       the argument and the open term separately and then composing the functions,
-       
-
-       then start working on 
-     *)
+Fixpoint equiv_type (t : type) : denote_type t -> denote_type t -> Prop :=
+  match t with 
+  | Nat => eq
+  | Pair t1 t2 => fun '(v1, v2) '(v3, v4) => equiv_type t1 v1 v3 /\ equiv_type t2 v2 v4
+  | Arrow t1 
 *)
+
+Equations var_map_weaken {Γ2} Γ1 (f : forall t, var t Γ1 -> var t Γ2) (hyps : denote_ctx Γ2) : denote_ctx Γ1 :=
+  var_map_weaken [] f hyps := tt;
+  var_map_weaken (t1 :: Γ1) f hyps :=
+    (index_ctx (f t1 VarZ) hyps, var_map_weaken Γ1 (fun t x => f t (VarS x))  hyps).
+Arguments var_map_weaken {_ _}.
+
+Lemma index_weaken:
+  forall (t : vtype) (Γ : ctx) (x : var t Γ) (Γ2 : ctx) (f : forall t' : vtype, var t' Γ -> var t' Γ2) (hyps : denote_ctx Γ2),
+    index_ctx (f t x) hyps = index_ctx x (var_map_weaken f hyps).
+Proof.
+  intros t Γ x Γ2 f hyps.
+  revert f hyps. induction Γ. inversion x. intros.
+  dependent destruction x.
+  - simp var_map_weaken. simp index_ctx. auto.
+  - simp var_map_weaken. simp index_ctx. setoid_rewrite <- IHΓ.
+    auto.
+Qed.
+
+Lemma var_map_weaken_skip:
+  forall (t1 : vtype) (Γ Γ2 : ctx) (f : forall t' : vtype, var t' Γ -> var t' Γ2) (hyps : denote_ctx Γ2) (v : denote_type t1),
+    var_map_weaken (var_map_skip f) (v, hyps) = (v, var_map_weaken f hyps).
+Proof.
+  intros t1 Γ Γ2 f hyps.
+  intros. simp var_map_weaken. simp index_ctx.
+  (* try to finish this, then write down desirata for type equiv*)
+  enough (var_map_weaken (fun (t : vtype) (x : var t Γ) => var_map_skip f t (VarS x)) (v, hyps) = var_map_weaken f hyps). subst. rewrite H. auto.
+  simp var_map_weaken.
+  generalize dependent v.  generalize dependent f.
+  generalize dependent hyps.
+  induction Γ.
+  - intros. cbn in hyps. simp var_map_weaken. auto.
+  - intros. specialize (IHΓ hyps (fun (t : vtype) (x : var t Γ) => f t (VarS x)) v). 
+    simp var_map_skip in IHΓ.
+    simp var_map_weaken. simp var_map_skip.
+    rewrite <- IHΓ. simp index_ctx. auto.
+Qed.
+
+(* comp_value_mutind *)
+Lemma comp_val_bodies_map : 
+  (forall t Γ1 MR (c : comp t Γ1 MR), forall Γ2 (f : forall t', var t' Γ1 -> var t' Γ2) 
+  (hyps : denote_ctx Γ2),
+  denote_comp (comp_map c f) hyps ≈ denote_comp c (var_map_weaken f hyps) ) /\
+  (forall t Γ1 (v : value t Γ1) MR Γ2  (f : forall t', var t' Γ1 -> var t' Γ2) 
+  (hyps : denote_ctx Γ2),
+  denote_value (MR := MR) (val_map v f) hyps ≈ denote_value v (var_map_weaken f hyps)) /\
+  (forall Γ1 MR R (bodies : mfix_bodies Γ1 MR R) Γ2 (f : forall t', var t' Γ1 -> var t' Γ2) 
+      (arg : denote_call_frame R)
+      (hyps : denote_ctx Γ2),
+  denote_bodies (bodies_map bodies f) hyps arg ≈ denote_bodies bodies (var_map_weaken f hyps) arg).
+Proof.
+  apply comp_value_mutind; intros; auto.
+  - rewrite val_map_equation_1. repeat rewrite denote_value_equation_1. 
+    reflexivity.
+  - rewrite val_map_equation_2. repeat rewrite denote_value_equation_2. reflexivity.
+  - rewrite val_map_equation_3. repeat rewrite denote_value_equation_3. rewrite H.
+    setoid_rewrite H0. reflexivity.
+  - rewrite val_map_equation_4. repeat rewrite denote_value_equation_4.
+    rewrite H. setoid_rewrite H0. reflexivity.
+  - rewrite val_map_equation_5. repeat rewrite denote_value_equation_5.
+    apply eqit_Ret. admit.
+  - rewrite val_map_equation_6. repeat rewrite denote_value_equation_6.
+    apply eqit_Ret. apply index_weaken.
+  - simp comp_map. simp denote_comp.
+  - simp comp_map. simp denote_comp. rewrite H. setoid_rewrite H0.
+    simp var_map_weaken.
+    assert (forall v : denote_type t1, var_map_weaken (var_map_skip f) (v, hyps) = (v, var_map_weaken f hyps)). apply var_map_weaken_skip; auto.
+    eapply eqit_bind. reflexivity. intros. subst. rewrite H1. reflexivity.
+  - simp comp_map. simp denote_comp.
+    rewrite H.
+    eapply eqit_bind. reflexivity. intros. subst.
+    destruct u2; eauto. eapply H0.
+    rewrite H1. rewrite var_map_weaken_skip. reflexivity.
+  - simp comp_map. simp denote_comp.
+    rewrite H. eapply eqit_bind. reflexivity.
+    intros. subst. destruct u2. eapply H0.
+    simp var_map_skip. 
+    specialize var_map_weaken_skip with (t1 := List t1) (v := u2) as H2.
+    rewrite <- H2.
+    specialize var_map_weaken_skip with (v := d) (Γ2 := List t1 :: Γ2) 
+      (hyps := (u2, hyps) ) (f := var_map_skip f) as H3.
+    setoid_rewrite <- H3. 
+    simp var_map_weaken. simp index_ctx. simp var_map_skip.
+    simp index_ctx. simp var_map_weaken.
+    admit. (* maybe there are better abstractions and lemmas for reasoning *)
+  - simp comp_map. simp denote_comp. rewrite H.
+    eapply eqit_bind. reflexivity. intros. subst. destruct u2.
+    (* similar to previous *) admit.
+  - simp comp_map. simp denote_comp. rewrite H.
+    eapply eqit_bind. reflexivity. intros. subst.
+    rewrite H0. reflexivity.
+  - simp comp_map. simp denote_comp. rewrite H. reflexivity.
+  - simp comp_map. simp denote_comp. setoid_rewrite H0.
+    (* think carefully about the relation here and might need another
+       properness for interp *)
+    admit.
+Admitted.
+
+Lemma comp_map_correct t Γ1 Γ2 MR (c : comp t Γ1 MR) (f : forall t', var t' Γ1 -> var t' Γ2) 
+  (hyps : denote_ctx Γ2) :
+  denote_comp (comp_map c f) hyps ≈ denote_comp c (var_map_weaken f hyps).
+Proof.
+  intros. destruct comp_val_bodies_map. auto.
+Qed.
+
+Lemma val_map_correct t Γ1 Γ2 MR (v : value t Γ1) (f : forall t', var t' Γ1 -> var t' Γ2) 
+  (hyps : denote_ctx Γ2) :
+  denote_value (MR := MR) (val_map v f) hyps ≈ denote_value v (var_map_weaken f hyps).
+Proof.
+  intros. destruct comp_val_bodies_map as [ ? [? ?] ]. auto.
+Qed.
+
+Lemma bodies_map_correct Γ1 Γ2 MR R (bodies : mfix_bodies Γ1 MR R) (f : forall t', var t' Γ1 -> var t' Γ2) 
+      (arg : denote_call_frame R)
+      (hyps : denote_ctx Γ2) : 
+  denote_bodies (bodies_map bodies f) hyps arg ≈ denote_bodies bodies (var_map_weaken f hyps) arg.
+Proof.
+  intros. destruct comp_val_bodies_map as [ ? [? ?] ]. auto.
+Qed.
+
+Equations insert_ctx {t Γ2} Γ1 (v : denote_type t) (hyps : denote_ctx (Γ1 ++ Γ2) ) : 
+  denote_ctx (Γ1 ++ [t] ++ Γ2) :=
+  insert_ctx [] v hyps := (v,hyps);
+  insert_ctx (t1 :: Γ1) v (v1, hyps) := (v1, insert_ctx Γ1 v hyps).
+Arguments insert_ctx {_ _ _}.
+Equations apply_middle {t Γ2 T} Γ1 (f : denote_ctx (Γ1 ++ [t] ++ Γ2 ) -> T) (v : denote_type t) 
+  (hyps : denote_ctx (Γ1 ++ Γ2) ) : T :=
+  apply_middle [] f v hyps := f (v,hyps);
+  apply_middle (t1 :: Γ1) f v (x,hyps) :=
+    apply_middle Γ1 (fun hyps' => f (x,hyps') ) v hyps.
+Arguments apply_middle {_ _ _ _}.
+
+Equations hyps_app {Γ2} Γ1 (hyps1 : denote_ctx Γ1) (hyps2 : denote_ctx Γ2) : denote_ctx (Γ1 ++ Γ2) :=
+  hyps_app [] _ hyps2 := hyps2;
+  hyps_app _ (v, hyps1) hyps2 := (v, hyps_app _ hyps1 hyps2).
+Arguments hyps_app {_ _}.
+Notation "h1 +++ h2" := (hyps_app h1 h2) (at level 30).
+
+
+
+
+Lemma subst_correct_aux t u Γ1 Γ2 MR (c : comp u (Γ1 ++ [t] ++ Γ2) MR)  : 
+  forall (v : value t Γ2) (hyps1 : denote_ctx Γ1) (hyps2 : denote_ctx Γ2) v',
+    denote_value (MR := MR) v hyps2 ≈ ret v' ->
+    denote_comp (subst_comp c v) (hyps1 +++ hyps2) ≈
+                denote_comp c (insert_ctx v' (hyps1 +++ hyps2)).
+Proof.
+  (* need dependent induction for compm value and subst,
+     will need reasoning principles for subst_var, and all of the weakings,
+     which means reasoning principle for comp_map
+*)
+  dependent induction c.
+Admitted.
+
+Theorem subst_correct t u Γ MR (c : comp u (t :: Γ) MR) (v : value t Γ) : 
+  forall (hyps : denote_ctx Γ) v',
+    denote_value (MR := MR) v hyps ≈ ret v' ->
+    denote_comp (subst_comp_cons c v) hyps ≈
+                denote_comp c (v', hyps).
+Proof.
+  intros. specialize (subst_correct_aux t u nil Γ MR c v tt _ _ H) as Heq.
+  simp hyps_app in Heq.
+Qed.
