theories/AlmostStlc/Syntax.v
@@ -1,15 +1,6 @@
 
 Require Export TypedVar.
-
-Inductive type : Type :=
-  | Nat : type
-  | List : type -> type
-  | Pair : type -> type -> type
-  | Arrow : type -> (list (list (type * type))) -> type -> type
-.
-Notation ctx := (list type).
-Notation call_frame := (list (type * type)).
-Notation mfix_ctx := (list call_frame).
+Require Export Types.
 
 
 
