theories/Eq/Rutt.v
@@ -12,8 +12,375 @@ From ITree Require Import
      Basics.HeterogeneousRelations
      Eq.Paco2.
 
+From ExtLib Require Import
+     Structures.Monad.
+
 From EnTree Require Import
      Basics.HeterogeneousRelations
-     Core.EnTreeDefinition.
+     Core.EnTreeDefinition
+     Eq.Eqit
+.
 
 Local Open Scope entree_scope.
+
+From Paco Require Import paco.
+
+Import Monads.
+Import MonadNotation.
+Local Open Scope monad_scope.
+Section RuttF.
+
+  Context {E1 E2 : Type} `{enc1 : EncodedType E1} `{enc2 : EncodedType E2}.
+  Context {R1 R2 : Type}.
+  Context (RPre : Rel E1 E2).
+  Context (RPost : PostRel E1 E2).
+  Context (RR : Rel R1 R2).
+
+  Inductive ruttF (sim : entree E1 R1 -> entree E2 R2 -> Prop) : entree' E1 R1 -> entree' E2 R2 -> Prop :=
+  | EqRet : forall (r1 : R1) (r2 : R2),
+      RR r1 r2 ->
+      ruttF sim (RetF r1) (RetF r2)
+  | EqTau : forall (m1 : entree E1 R1) (m2 : entree E2 R2),
+      sim m1 m2 ->
+      ruttF sim (TauF m1) (TauF m2)
+  | EqVis : forall (e1 : E1) (e2 : E2) (k1 : encodes e1 -> entree E1 R1) (k2 : encodes e2 -> entree E2 R2),
+      RPre e1 e2 ->
+      (forall a b, RPost e1 e2 a b -> sim (k1 a) (k2 b)) ->
+      ruttF sim (VisF e1 k1) (VisF e2 k2)
+  | EqTauL : forall (t1 : entree E1 R1) (ot2 : entree' E2 R2),
+      ruttF sim (observe t1) ot2 ->
+      ruttF sim (TauF t1) ot2
+  | EqTauR : forall (ot1 : entree' E1 R1) (t2 : entree E2 R2),
+      ruttF sim ot1 (observe t2) ->
+      ruttF sim ot1 (TauF t2).
+  Hint Constructors ruttF : entree.
+  
+  Definition rutt_ sim t1 t2 := ruttF sim (observe t1) (observe t2).
+  Hint Unfold rutt_ : entree.
+
+  Lemma rutt_monot : monotone2 rutt_.
+  Proof.
+    red. intros. red. induction IN; eauto with entree.
+  Qed.
+
+  Definition rutt : entree E1 R1 -> entree E2 R2 -> Prop := paco2 rutt_ bot2.
+
+  Lemma ruttF_inv_VisF_r {sim} t1 (e2: E2) (k2: encodes e2 -> _):
+    ruttF sim t1 (VisF e2 k2) ->
+    (exists (e1: E1) k1, t1 = VisF e1 k1 /\
+      forall v1 v2, RPost e1 e2 v1 v2 -> sim (k1 v1) (k2 v2))
+    \/
+    (exists t1', t1 = TauF t1' /\
+      ruttF sim (observe t1') (VisF e2 k2)).
+  Proof.
+    refine (fun H =>
+      match H in ruttF _ _ t2 return
+        match t2 return Prop with
+        | VisF e2 k2 => _
+        | _ => True
+        end
+      with
+      | EqVis _ _ _ _ _ _ _ => _
+      | _ => _
+      end); try exact I.
+    - left; eauto.
+    - destruct e0; eauto.
+  Qed.
+
+  Lemma ruttF_inv_VisF {sim}
+      (e1 : E1) (e2 : E2) (k1 : encodes e1 -> _) (k2 : encodes e2 -> _)
+    : ruttF sim (VisF e1 k1) (VisF e2 k2) ->
+      forall v1 v2, RPost e1 e2 v1 v2 -> sim (k1 v1) (k2 v2).
+  Proof.
+    intros H. dependent destruction H. assumption.
+  Qed.
+
+
+  Ltac unfold_rutt :=
+    (try match goal with [|- rutt_ _ _ _ _ _ _ _ ] => red end);
+    (repeat match goal with [H: rutt_ _ _ _ _ _ _ _ |- _ ] => red in H end).
+
+  Lemma fold_ruttF:
+    forall (t1: entree E1 R1) (t2: entree E2 R2) ot1 ot2,
+    ruttF (upaco2 rutt_ bot2) ot1 ot2 ->
+    ot1 = observe t1 ->
+    ot2 = observe t2 ->
+    rutt t1 t2.
+  Proof.
+    intros * eq -> ->; pfold; auto.
+  Qed.
+End RuttF.
+
+Tactic Notation "fold_ruttF" hyp(H) :=
+  try punfold H;
+  try red in H;
+  match type of H with
+  | ruttF ?_REV ?_RANS ?_RR (upaco2 (rutt_ ?_REV ?_RANS ?_RR) bot2) ?_OT1 ?_OT2 =>
+      match _OT1 with
+      | observe _ => idtac
+      | ?_OT1 => rewrite (entree_eta' _OT1) in H
+      end;
+      match _OT2 with
+      | observe _ => idtac
+      | ?_OT2 => rewrite (entree_eta' _OT2) in H
+      end;
+      eapply fold_ruttF in H; [| eauto | eauto]
+  end.
+
+
+#[global] Hint Resolve rutt_monot : paco.
+
+Section ConstructionInversion.
+  Context (E1 E2 : Type) `{enc1 : EncodedType E1} `{enc2 : EncodedType E2}.
+  Context (R1 R2 : Type).
+  Context (RPre : Rel E1 E2).
+  Context (RPost : PostRel E1 E2).
+  Context (RR : Rel R1 R2).
+
+Lemma rutt_Ret r1 r2:
+  RR r1 r2 ->
+  rutt RPre RPost RR (Ret r1) (Ret r2).
+Proof. intros. pstep; constructor; auto. Qed.
+
+Lemma rutt_inv_Ret r1 r2:
+  rutt RPre RPost RR (Ret r1) (Ret r2) -> RR r1 r2.
+Proof.
+  intros. punfold H. inv H. eauto.
+Qed.
+
+Lemma rutt_inv_Ret_l r1 t2:
+  rutt RPre RPost RR (Ret r1) t2 -> exists r2, t2 ≳ Ret r2 /\ RR r1 r2.
+Proof.
+  intros Hrutt; punfold Hrutt; red in Hrutt; cbn in Hrutt.
+  setoid_rewrite (entree_eta t2). remember (RetF r1) as ot1; revert Heqot1.
+  induction Hrutt; intros; try discriminate.
+  - inversion Heqot1; subst. exists r2. split; [reflexivity|auto].
+  - destruct (IHHrutt Heqot1) as [r2 [H1 H2]]. exists r2; split; auto.
+    rewrite <- entree_eta in H1. now rewrite tau_euttge.
+Qed.  
+
+Lemma rutt_inv_Ret_r t1 r2:
+  rutt RPre RPost RR t1 (Ret r2) -> exists r1, t1 ≳ Ret r1 /\ RR r1 r2.
+Proof.
+  intros Hrutt; punfold Hrutt; red in Hrutt; cbn in Hrutt.
+  setoid_rewrite (entree_eta t1). remember (RetF r2) as ot2; revert Heqot2.
+  induction Hrutt; intros; try discriminate.
+  - inversion Heqot2; subst. exists r1. split; [reflexivity|auto].
+  - destruct (IHHrutt Heqot2) as [r1 [H1 H2]]. exists r1; split; auto.
+    rewrite <- entree_eta in H1. now rewrite tau_euttge.
+Qed.
+
+Lemma rutt_inv_Tau_l t1 t2 :
+  rutt RPre RPost RR (Tau t1) t2 -> rutt RPre RPost RR t1 t2.
+Proof.
+  intros. punfold H. red in H. simpl in *.
+  remember (TauF t1) as tt1. genobs t2 ot2.
+  hinduction H before t1; intros; try discriminate.
+  - inv Heqtt1. pclearbot. pstep. red. simpobs. econstructor; eauto. pstep_reverse.
+  - inv Heqtt1. punfold_reverse H.
+  - red in IHruttF. pstep. red; simpobs. econstructor; eauto. pstep_reverse.
+Qed.
+
+Lemma rutt_add_Tau_l t1 t2 :
+  rutt RPre RPost RR t1 t2 -> rutt RPre RPost RR (Tau t1) t2.
+Proof.
+  intros. pfold. red. cbn. constructor. pstep_reverse.
+Qed.
+
+Lemma rutt_inv_Tau_r t1 t2 :
+  rutt RPre RPost RR t1 (Tau t2) -> rutt RPre RPost RR t1 t2.
+Proof.
+  intros. punfold H. red in H. simpl in *.
+  pstep. red. remember (TauF t2) as tt2 eqn:Ett2 in H.
+  revert t2 Ett2; induction H; try discriminate; intros; inversion Ett2; subst; auto.
+  - pclearbot. constructor. pstep_reverse.
+  - constructor. eapply IHruttF; eauto.
+Qed.
+
+Lemma rutt_add_Tau_r t1 t2 :
+  rutt RPre RPost RR t1 t2 -> rutt RPre RPost RR t1 (Tau t2).
+Proof.
+  intros. pfold. red. cbn. constructor. pstep_reverse.
+Qed.
+
+Lemma rutt_inv_Tau t1 t2 :
+  rutt RPre RPost RR (Tau t1) (Tau t2) -> rutt RPre RPost RR t1 t2.
+Proof.
+  intros; apply rutt_inv_Tau_r, rutt_inv_Tau_l; assumption.
+Qed.
+
+Lemma rutt_Vis (e1: E1) (e2: E2)
+    (k1: encodes e1 -> entree E1 R1) (k2: encodes e2 -> entree E2 R2):
+  RPre e1 e2 ->
+  (forall a b, RPost e1 e2 a b -> rutt RPre RPost RR (k1 a) (k2 b)) ->
+  rutt RPre RPost RR (Vis e1 k1) (Vis e2 k2).
+Proof.
+  intros He Hk. pstep; constructor; auto.
+  intros; left. apply Hk; auto.
+Qed.
+
+Lemma rutt_inv_Vis_l (e1: E1) k1 t2:
+  rutt RPre RPost RR (Vis e1 k1) t2 ->
+  exists (e2: E2) k2,
+    t2 ≈ Vis e2 k2 /\
+    RPre e1 e2 /\
+    (forall v1 v2, RPost e1 e2 v1 v2 -> rutt RPre RPost RR (k1 v1) (k2 v2)).
+Proof.
+  intros Hrutt; punfold Hrutt; red in Hrutt; cbn in Hrutt.
+  setoid_rewrite (entree_eta t2). remember (VisF e1 k1) as ot1; revert Heqot1.
+  induction Hrutt; intros; try discriminate; subst.
+  - inversion Heqot1. subst. inversion_sigma; rewrite <- eq_rect_eq in *;
+    subst. exists e2. exists k2. split. reflexivity. split; auto.
+    intros v1 v2 HAns. specialize (H0 v1 v2 HAns). red in H0. now pclearbot.
+  - destruct (IHHrutt eq_refl) as (e2 & k2 & Ht0 & HAns).
+    rewrite <- entree_eta in Ht0.
+    exists e2, k2; split; auto. now rewrite tau_eutt.
+Qed.
+
+Lemma rutt_inv_Vis_r t1 (e2: E2) k2:
+  rutt RPre RPost RR t1 (Vis e2 k2) ->
+  exists (e1: E1) k1,
+    t1 ≈ Vis e1 k1 /\
+    RPre e1 e2 /\
+    (forall v1 v2, RPost e1 e2 v1 v2 -> rutt RPre RPost RR (k1 v1) (k2 v2)).
+Proof.
+  intros Hrutt; punfold Hrutt; red in Hrutt; cbn in Hrutt.
+  setoid_rewrite (entree_eta t1). remember (VisF e2 k2) as ot2; revert Heqot2.
+  induction Hrutt; intros; try discriminate; subst.
+  - inversion Heqot2; subst. inversion_sigma; rewrite <- eq_rect_eq in *;
+    subst.
+    exists e1, k1; split. reflexivity. split; auto.
+    intros v1 v2 HAns. specialize (H0 v1 v2 HAns). red in H0. now pclearbot.
+  - destruct (IHHrutt eq_refl) as (e1 & k1 & Ht0 & HAns).
+    rewrite <- entree_eta in Ht0.
+    exists e1, k1; split; auto. now rewrite tau_eutt.
+Qed.
+
+Lemma rutt_inv_Vis  (e1: E1) (e2: E2)
+    (k1: encodes e1 -> entree E1 R1) (k2: encodes e2 -> entree E2 R2):
+  rutt RPre RPost RR (Vis e1 k1) (Vis e2 k2) ->
+  forall u1 u2, RPost e1 e2 u1 u2 -> rutt RPre RPost RR (k1 u1) (k2 u2).
+Proof.
+  intros H u1 u2 Hans. punfold H.
+  apply ruttF_inv_VisF with (v1 := u1) (v2 := u2) in H. pclearbot; auto.
+  assumption.
+Qed.
+
+
+End ConstructionInversion.
+
+Section euttge_trans_clo.
+
+  Context {E1 E2 : Type} `{enc1 : EncodedType E1} `{enc2 : EncodedType E2} {R1 R2 : Type} (RR : R1 -> R2 -> Prop).
+
+  (* Closing a relation over itrees under [euttge].
+     Essentially the same closure as [eqit_trans_clo], but heterogeneous
+     in the interface argument [E].
+     We only define the closure under [euttge] as opposed to [eqit_trans_clo]
+     capturing closure under [eq_itree] and [eutt] at the same time, since it's
+     the only one we need.
+   *)
+
+  (* A transitivity functor *)
+  Variant euttge_trans_clo (r : entree E1 R1 -> entree E2 R2 -> Prop) :
+    entree E1 R1 -> entree E2 R2 -> Prop :=
+    eqit_trans_clo_intro t1 t2 t1' t2' RR1 RR2
+                         (EQVl: euttge RR1 t1 t1')
+                         (EQVr: euttge RR2 t2 t2')
+                         (REL: r t1' t2')
+                         (LERR1: forall x x' y, RR1 x x' -> RR x' y -> RR x y)
+                         (LERR2: forall x y y', RR2 y y' -> RR x y' -> RR x y) :
+      euttge_trans_clo r t1 t2.
+  Hint Constructors euttge_trans_clo : itree.
+
+  Lemma euttge_trans_clo_mon r1 r2 t1 t2
+        (IN : euttge_trans_clo r1 t1 t2)
+        (LE : r1 <2= r2) :
+    euttge_trans_clo r2 t1 t2.
+  Proof.
+    destruct IN; econstructor; eauto.
+  Qed.
+
+  Hint Resolve euttge_trans_clo_mon : paco.
+
+End euttge_trans_clo.
+
+Lemma euttge_trans_clo_wcompat E1 E2 `{EncodedType E1} `{EncodedType E2} 
+      (RPre : Rel E1 E2) (RPost : PostRel E1 E2)
+      R1 R2 (RR : R1 -> R2 -> Prop) :
+  wcompatible2 (rutt_ RPre RPost RR) (euttge_trans_clo RR).
+Proof.
+  constructor; eauto with paco.
+  { red. intros. eapply euttge_trans_clo_mon; eauto. }
+  intros.
+  destruct PR. punfold EQVl. punfold EQVr. unfold_eqit.
+  hinduction REL before r; intros; clear t1' t2'.
+  - remember (RetF r1) as x. red.
+    hinduction EQVl before r; intros; subst; try inv Heqx; eauto; (try constructor; eauto).
+    remember (RetF r3) as x. hinduction EQVr before r; intros; subst; try inv Heqx; (try constructor; eauto).
+  - red. remember (TauF m1) as x.
+    hinduction EQVl before r; intros; subst; try inv Heqx; try inv CHECK; ( try (constructor; eauto; fail )).
+    remember (TauF m3) as y.
+    hinduction EQVr before r; intros; subst; try inv Heqy; try inv CHECK; (try (constructor; eauto; fail)).
+    pclearbot. constructor. gclo. econstructor; eauto with paco.
+  - remember (VisF e1 k1) as x. red.
+    hinduction EQVl before r; intros; subst; try discriminate; try (constructor; eauto; fail).
+    remember (VisF e2 k3) as y.
+    hinduction EQVr before r; intros; subst; try discriminate; try (constructor; eauto; fail).
+    dependent destruction Heqx.
+    dependent destruction Heqy.
+    constructor; auto. intros. apply H2 in H3. pclearbot.
+    apply gpaco2_clo.
+    econstructor; eauto with entree.
+  - remember (TauF t1) as x. red.
+    hinduction EQVl before r; intros; subst; try inv Heqx; try inv CHECK; (try (constructor; eauto; fail)).
+    pclearbot. punfold REL. constructor. eapply IHREL; eauto.
+  - remember (TauF t2) as y. red.
+    hinduction EQVr before r; intros; subst; try inv Heqy; try inv CHECK; (try (constructor; eauto; fail)).
+    pclearbot. punfold REL. constructor. eapply IHREL; eauto.
+Qed.
+
+#[global] Hint Resolve euttge_trans_clo_wcompat : paco.
+
+(* The validity of the up-to [euttge] entails we can rewrite under [euttge]
+   and hence also [eq_itree] during coinductive proofs of [rutt]
+*)
+#[global] Instance grutt_cong_eqit {R1 R2 : Type} {E1 E2 : Type} `{EncodedType E1} `{EncodedType E2} 
+ {RPre : Rel E1 E2} {RPost : PostRel E1 E2}
+       {RR1 RR2} {RS : R1 -> R2 -> Prop} r rg
+       (LERR1: forall x x' y, (RR1 x x': Prop) -> (RS x' y: Prop) -> RS x y)
+       (LERR2: forall x y y', (RR2 y y': Prop) -> RS x y' -> RS x y) :
+  Proper (eq_itree RR1 ==> eq_itree RR2 ==> flip impl)
+         (gpaco2 (rutt_ RPre RPost RS) (euttge_trans_clo RS) r rg).
+Proof.
+  repeat intro. gclo. econstructor; eauto;
+    try eapply eqit_mon; try apply H1; try apply H2; auto with entree.
+Qed.
+
+Global Instance grutt_cong_euttge {R1 R2 : Type} {E1 E2 : Type} `{EncodedType E1} `{EncodedType E2} 
+ {RPre : Rel E1 E2} {RPost : PostRel E1 E2} {RR1 RR2} {RS : R1 -> R2 -> Prop} r rg
+       (LERR1: forall x x' y, (RR1 x x': Prop) -> (RS x' y: Prop) -> RS x y)
+       (LERR2: forall x y y', (RR2 y y': Prop) -> RS x y' -> RS x y) :
+  Proper (euttge RR1 ==> euttge RR2 ==> flip impl)
+         (gpaco2 (rutt_ RPre RPost RS) (euttge_trans_clo RS) r rg).
+Proof.
+  repeat intro. gclo. econstructor; eauto.
+Qed.
+
+(* Provide these explicitly since typeclasses eauto cannot infer them *)
+
+#[global] Instance grutt_cong_eqit_eq {R1 R2 : Type} {E1 E2 : Type} `{EncodedType E1} `{EncodedType E2} 
+ {RPre : Rel E1 E2} {RPost : PostRel E1 E2} {RS : R1 -> R2 -> Prop} r rg:
+    Proper (eq_itree eq ==> eq_itree eq ==> flip impl)
+         (gpaco2 (rutt_ RPre RPost RS) (euttge_trans_clo RS) r rg).
+Proof.
+  apply grutt_cong_eqit; now intros * ->.
+Qed.
+
+#[global] Instance grutt_cong_euttge_eq {R1 R2 : Type} {E1 E2 : Type} `{EncodedType E1} `{EncodedType E2} 
+ {RPre : Rel E1 E2} {RPost : PostRel E1 E2} {RS : R1 -> R2 -> Prop} r rg:
+    Proper (euttge eq ==> euttge eq ==> flip impl)
+         (gpaco2 (rutt_ RPre RPost RS) (euttge_trans_clo RS) r rg).
+Proof.
+  apply grutt_cong_euttge; now intros * ->.
+Qed.
