theories/AlmostStlc/DenotationSeq.v
@@ -1,0 +1,74 @@
+Require Export MrecMonad.
+Require Export HeterogeneousRelations.
+Require Export EnTreeDefinition.
+Require Export Denotation.
+Require Export SyntaxSeq.
+From Coq Require Import Lists.List Logic.JMeq.
+
+From Equations Require Import Equations Signature.
+
+Import Monads.
+Import MonadNotation.
+Local Open Scope monad_scope.
+
+
+Equations denote_comp {t Γ MR} (c : comp t Γ MR) (hyps : denote_ctx Γ) :
+  mtree (denote_mfix_ctx MR) (denote_type t) := {
+    denote_comp (comp_ret v) hyps := denote_value v hyps;
+    denote_comp (comp_let c1 c2) hyps :=
+      v <- denote_comp c1 hyps;;
+      denote_comp c2 (v,hyps);
+    denote_comp (comp_match_nat vn eZ eS) hyps :=
+      n <- denote_value vn hyps;;
+      match n with
+      | 0 => denote_comp eZ hyps
+      | S m => denote_comp eS (m, hyps)
+      end;
+    denote_comp (comp_match_list vl enil econs) hyps :=
+      l <- denote_value vl hyps;;
+      match l with
+      | nil => denote_comp enil hyps
+      | h :: t => denote_comp econs (h, (t, hyps))
+      end;
+    denote_comp (comp_split vp es) hyps :=
+      '(v1,v2) <- denote_value vp hyps;;
+      denote_comp es (v1, (v2, hyps));
+    denote_comp (comp_app vf varg) hyps :=
+      vf' <- denote_value vf hyps;;
+      varg' <- denote_value varg hyps;;
+      vf' varg';
+    denote_comp (comp_call xR x varg) hyps :=
+      varg' <- denote_value varg hyps;;
+      call_term x xR varg';
+    denote_comp (comp_lift c) hyps :=
+      mapE lift_handler (denote_comp c hyps);
+    denote_comp (comp_perm Hperm c) hyps :=
+      map_perm _ _ (perm_denote Hperm) (denote_comp c hyps);
+    denote_comp (comp_mfix xR bodies c) hyps := 
+    mapE (remove_denote xR) 
+         (interp_mtree _ _ _ (denote_var xR) (denote_bodies bodies hyps) (denote_comp c hyps));
+  }
+where denote_value {t Γ MR} (v : value t Γ) (hyps : denote_ctx Γ) : 
+  mtree (denote_mfix_ctx MR) (denote_type t) := {
+    denote_value (val_const n) _ := ret n;
+    denote_value val_nil _ := ret nil;
+    denote_value (val_cons vh vt) hyps :=
+      vh' <- denote_value vh hyps;;
+      vt' <- denote_value vt hyps;;
+      ret (cons vh' vt');
+    denote_value (val_pair v1 v2) hyps :=
+      v1' <- denote_value v1 hyps;;
+      v2' <- denote_value v2 hyps;;
+      ret (v1',v2');
+    denote_value (val_abs cbody) hyps :=
+      ret (fun x => denote_comp cbody (x,hyps));
+    denote_value (val_var x) hyps := ret (index_ctx x hyps);
+}
+where denote_bodies {Γ MR R} (bodies : mfix_bodies Γ MR R) 
+                    (hyps : denote_ctx Γ) (arg : denote_call_frame R)  : 
+  mtree (denote_mfix_ctx MR) (encodes arg) := {
+  denote_bodies (mfix_bodies_cons body _) hyps (inl arg) :=
+    denote_comp body (arg, hyps);
+  denote_bodies (mfix_bodies_cons _ bodies) hyps (inr arg) :=
+    denote_bodies bodies hyps arg
+}.
