theories/AlmostStlc/Types.v
@@ -1,0 +1,11 @@
+Inductive type : Type :=
+  | Nat : type
+  | List : type -> type
+  | Pair : type -> type -> type
+  | Arrow : type -> (list (list (type * type))) -> type -> type
+.
+Notation ctx := (list type).
+Notation call_frame := (list (type * type)).
+Notation mfix_ctx := (list call_frame).
+
+Notation vtype := type.
