theories/AlmostStlc/TypesEquiv.v
@@ -1,0 +1,121 @@
+Require Export TypedVar.
+Require Export SyntaxSeq.
+Require Export SmallStepSeq.
+Require Export DenotationFacts.
+Require Export DenotationSeq.
+Require Export Rutt.
+Require Export RuttFacts.
+Require Import ITree.Basics.HeterogeneousRelations.
+Import List.ListNotations.
+Open Scope list_scope.
+From Equations Require Import Equations Signature.
+Require Import Coq.Program.Equality.
+Require Import ExtLib.Structures.Monad.
+Import MonadNotation.
+Local Open Scope monad_scope.
+
+Inductive list_rel {A} (R : Rel A A): Rel (list A) (list A) :=
+  | list_rel_nil : list_rel R nil nil
+  | list_rel_cons a b l1 l2 : R a b ->list_rel R l1 l2 -> list_rel R (cons a l1) (cons a l2).
+
+Section types_equiv.
+
+(*
+
+Inductive types_equiv : forall t : type, Rel (denote_type t) (denote_type t) := 
+  | types_equiv_Nat n : types_equiv Nat n n
+  | types_equiv_Pair t1 t2 p1 p2 : prod_rel (types_equiv t1) (types_equiv t2) p1 p2 ->
+                                   types_equiv (Pair t1 t2) p1 p2
+  | types_equiv_List t l1 l2 : list_rel (types_equiv t) l1 l2 ->
+                               types_equiv (List t) l1 l2
+  | types_equiv_Arrow t1 MR t2 f g : 
+    (forall x y, types_equiv t1 x y -> rutt hole hole (types_equiv t2) (f x) (g x) ) ->
+    types_equiv (Arrow t1 MR t2) f g
+.
+the arrow type requires non strict positive application, needs to be a fixpoint
+
+
+*)
+
+(* seems to not be recognizing  that this is well founded, probably a dependent 
+   pattern matching problem, first thing to try might be to do this in equations
+   after that maybe consider some gas-like solution
+
+   this might take much of tomorrow, I am concerned about the march deadline,
+   but if we miss it thats not really a problem talk about the next deadline with steve next week
+
+  *)
+(* maybe also create a generalized version of this so that we can get some more 
+   general equational theory working 
+   maybe also a relation for any mtree, built on top of rutt and do some of the 
+   theory at that level
+*)
+Equations types_equiv (t : type) : Rel (denote_type t) (denote_type t) := {
+    types_equiv Nat := eq;
+    types_equiv (Pair t1 t2) := prod_rel (types_equiv t1) (types_equiv t2);
+    types_equiv (List t) := list_rel (types_equiv t);
+    types_equiv (Arrow t1 MR t2) :=
+    fun f g => forall x y, types_equiv t1 x y -> 
+                   rutt (mfix_pre_equiv MR) (mfix_post_equiv MR) (types_equiv t2) (f x) (g y)
+}
+where mfix_pre_equiv (MR : mfix_ctx) : 
+  Rel (denote_mrec_ctx (denote_mfix_ctx MR)) (denote_mrec_ctx (denote_mfix_ctx MR)) :=
+{
+  mfix_pre_equiv nil := fun _ _ => False;
+  mfix_pre_equiv (cons cf MR) :=
+    sum_rel (call_frame_pre_equiv cf) (mfix_pre_equiv MR);
+}
+where call_frame_pre_equiv (cf : call_frame) :
+  Rel (denote_call_frame cf) (denote_call_frame cf) := 
+{
+  call_frame_pre_equiv nil := fun _ _ => False;
+  call_frame_pre_equiv (cons (t1,t2) cf') :=
+    sum_rel (types_equiv t1) (call_frame_pre_equiv cf')
+}
+where mfix_post_equiv (MR : mfix_ctx) : 
+  PostRel (denote_mrec_ctx (denote_mfix_ctx MR)) (denote_mrec_ctx (denote_mfix_ctx MR)) :=
+{
+  mfix_post_equiv nil := fun _ _ _ _ => False;
+  mfix_post_equiv (cons cf MR) := SumPostRel (call_frame_post_equiv cf) (mfix_post_equiv MR);
+}
+where call_frame_post_equiv (cf : call_frame) : 
+  PostRel (denote_call_frame cf) (denote_call_frame cf) :=
+{
+  call_frame_post_equiv nil := fun _ _ _ _ => False;
+  call_frame_post_equiv (cons (t1,t2) cf ) :=
+    SumPostRel (fun _ _ => types_equiv t2) (call_frame_post_equiv cf);
+}.
+(* use to create relations for [Γ] -> mtree [MR] [t] *)
+
+Fixpoint ctx_equiv (Γ : ctx) : Rel (denote_ctx Γ) (denote_ctx Γ) :=
+  match Γ with
+  | nil => fun _ _ => True
+  | cons t Γ => prod_rel (types_equiv t) (ctx_equiv Γ)
+  end.
+
+Definition comp_equiv {t Γ MR} :=
+    fun c1 c2 => forall hyps1 hyps2, ctx_equiv Γ hyps1 hyps2 ->
+              rutt (mfix_pre_equiv MR) (mfix_post_equiv MR) (types_equiv t) (c1 hyps1) (c2 hyps2).
+
+
+(*
+Should be a PER 
+
+
+rewrite with eutt
+
+it should generalize eutt
+
+should be the case that if it is a denotation, then it is self related
+so it acts as an equivalence relation on its actual domain
+
+
+tomorrow would be a good time to get a basic sketch of rutt done at least,
+leave implementations of lemmas for later, there is a sense in which it is not
+along a critical path because it is known to be true, where as
+other things might actually include some bugs
+
+on monday work on this but also dedicate some time to the proposal intro
+
+
+*)
