theories/Eq/RuttFacts.v
@@ -1,0 +1,295 @@
+From Coq Require Import
+     Program
+     Setoid
+     Morphisms
+     RelationClasses.
+
+From Paco Require Import paco.
+
+From ITree Require Import
+     Basics.Basics
+     Basics.Tacs
+     Basics.HeterogeneousRelations
+     Eq.Paco2.
+
+From ExtLib Require Import
+     Structures.Monad.
+
+From EnTree Require Import
+     Basics.HeterogeneousRelations
+     Core.EnTreeDefinition
+     Core.SubEvent
+     Eq.Eqit
+     Eq.Rutt
+.
+
+Local Open Scope entree_scope.
+
+From Paco Require Import paco.
+
+Import Monads.
+Import MonadNotation.
+Local Open Scope monad_scope.
+
+Lemma rutt_trigger {E1 E2} `{EncodedType E1} `{EncodedType E2}
+      (RPre : Rel E1 E2) (RPost : PostRel E1 E2) 
+      (e1: E1) (e2: E2) (RR : Rel (encodes e1) (encodes e2) ):
+  RPre e1 e2 ->
+  (forall a b, RPost e1 e2 a b -> RR a b) ->
+  rutt RPre RPost RR (EnTree.trigger e1) (EnTree.trigger e2).
+Proof.
+  intros. apply rutt_Vis; auto.
+  intros. apply rutt_Ret; auto.
+Qed.
+
+Lemma rutt_flip {E1 E2 R1 R2} `{enc1 : EncodedType E1} `{enc2 : EncodedType E2} 
+      RPre RPost RR (t1: entree E1 R1) (t2: entree E2 R2):
+  rutt RPre RPost RR t1 t2 <-> rutt (flip RPre) (FlipPostRel RPost) (flip RR) t2 t1.
+Proof.
+  split; revert t1 t2; pcofix CIH; intros t1 t2 Hrutt;
+  punfold Hrutt; red in Hrutt; pstep; red.
+  - induction Hrutt; try now constructor.
+    * apply EqTau. right. apply CIH. now pclearbot.
+    * apply EqVis. auto. intros b a HAns. cbn in HAns. right.
+      specialize (H0 a b HAns). apply CIH. now pclearbot.
+  - induction Hrutt; try now constructor.
+    * apply EqTau. right. apply CIH. now pclearbot.
+    * apply EqVis. auto. intros b a HAns. cbn in HAns. right.
+      specialize (H0 a b HAns). apply CIH. now pclearbot.
+Qed.
+
+
+(* Progressive [Proper] instances for [rutt] and congruence with eutt. *)
+
+#[global] Instance rutt_Proper_R {E1 E2 R1 R2} `{enc1 : EncodedType E1} 
+ `{enc2 : EncodedType E2} :
+  Proper (eq_rel         (* REv *)
+      ==> PostRelEq       (* RAns *)
+      ==> @eq_rel R1 R2  (* RR *)
+      ==> eq             (* t1 *)
+      ==> eq             (* t2 *)
+      ==> iff) (@rutt E1 E2 enc1 enc2 R1 R2).
+Proof.
+  intros REv1 REv2 HREv  RAns1 RAns2 HRAns RR1 RR2 HRR t1 _ <- t2 _ <-.
+  split; intros Hrutt.
+
+  - revert t1 t2 Hrutt; pcofix CIH; intros t1 t2 Hrutt.
+    pstep. punfold Hrutt. red in Hrutt; red.
+    hinduction Hrutt before CIH; intros; eauto with entree.
+    * apply EqRet. now apply HRR.
+    * apply EqTau. right. apply CIH. now pclearbot.
+    * apply EqVis. now apply HREv. intros.
+      assert (H2: RAns1 e1 e2 a b).
+      { apply  HRAns. auto. }
+      intros. specialize (H0 a b H2). red. right. apply CIH.
+      red in H0. now pclearbot.
+    * constructor. auto.
+    * constructor. auto.
+  - revert t1 t2 Hrutt; pcofix CIH; intros t1 t2 Hrutt.
+    pstep. punfold Hrutt. red in Hrutt; red.
+    hinduction Hrutt before CIH; intros; eauto.
+    * apply EqRet. now apply HRR.
+    * apply EqTau. right. apply CIH. now pclearbot.
+    * apply EqVis. now apply HREv. intros.
+      assert (H2: RAns2 e1 e2 a b).
+      { apply HRAns. auto. }
+      intros. specialize (H0 a b H2). red. right. apply CIH.
+      red in H0. now pclearbot.
+   * constructor. auto.
+   * constructor. auto.
+Qed.
+(*
+#[global] Instance rutt_Proper_R' {E1 E2 R1 R2} `{enc1 : EncodedType E1} 
+ `{enc2 : EncodedType E2} :
+  Proper (eq_rel         (* REv *)
+      ==> PostRelEq       (* RAns *)
+      ==> @eq_rel R1 R2  (* RR *)
+      ==> eq             (* t1 *)
+      ==> eq             (* t2 *)
+      ==> flip impl) (@rutt E1 E2 enc1 enc2 R1 R2).
+Proof.
+*)
+#[global] Instance rutt_Proper_R2 {E1 E2 R1 R2}  `{enc1 : EncodedType E1} 
+ `{enc2 : EncodedType E2}:
+  Proper (eq_rel         (* REv *)
+      ==> PostRelEq        (* RAns *)
+      ==> @eq_rel R1 R2  (* RR *)
+      ==> eq_itree eq    (* t1 *)
+      ==> eq_itree eq    (* t2 *)
+      ==> iff) (@rutt E1 E2 enc1 enc2 R1 R2).
+Proof.
+  clear. intros REv1 REv2 HREv RAns1 RAns2 HRAns RR1 RR2 HRR t1 t1' Ht1 t2 t2' Ht2.
+  split; intros Hrutt.
+  - rewrite  <- HREv, <- HRAns, <- HRR; clear HREv REv2 HRAns RAns2 HRR RR2.
+    ginit. gclo. econstructor; eauto with paco.
+    * symmetry in Ht1. apply eq_sub_euttge in Ht1. apply Ht1.
+    * symmetry in Ht2. apply eq_sub_euttge in Ht2. apply Ht2.
+    * intros; now subst.
+    * intros; now subst.
+  - rewrite HREv, HRAns, HRR; clear HREv REv1 HRAns RAns1 HRR RR1.
+    ginit. gclo. econstructor; eauto with paco.
+    * apply eq_sub_euttge in Ht1. apply Ht1.
+    * apply eq_sub_euttge in Ht2. apply Ht2.
+    * intros; now subst.
+    * intros; now subst.
+Qed.
+
+(* this should be one of the main goals of today*)
+Lemma rutt_cong_eutt {E1 E2 R1 R2} `{enc1 : EncodedType E1} `{enc2 : EncodedType E2} :
+  forall RPre RPost RR (t1: entree E1 R1) t1' (t2: entree E2 R2),
+  rutt RPre RPost RR t1 t2 ->
+  t1 ≈ t1' ->
+  rutt RPre RPost RR t1' t2.
+Proof.
+  (* First by coinduction; then do an induction on Hrutt to expose the ruttF
+     linking t1 and t2; then an induction on Heutt to expose the relation
+     between t1 and t1'. Finally, explore ruttF until landing on an rutt where
+     the t1/t1' relation can be substituted by CIH, and conclude. *)
+  intros * Hrutt Heutt; revert t1 t1' Heutt t2 Hrutt.
+  ginit; gcofix CIH; intros t1 t1' Heutt t2 Hrutt.
+  punfold Hrutt; red in Hrutt.
+  rewrite (entree_eta t1) in Heutt.
+  rewrite (entree_eta t2).
+
+  move Hrutt before CIH; revert_until Hrutt.
+  induction Hrutt as [r1 r2|m1 m2| |m1 ot2|]; clear t1 t2; intros t1' Heutt.
+
+  (* EqRet: t1 = Ret r1 ≈ t1'; we can rewrite away the Taus with the euttge
+     closure and finish immediately with EqRet. *)
+  * apply eutt_inv_Ret_l in Heutt. rewrite Heutt.
+    gfinal; right; pstep. now apply EqRet.
+
+  (* EqTau: The hardest case. When Heutt is EqTauL then we lack information to
+     proceed, which requires that [desobs m1]. We then have to restart
+     analyzing based on m1; the Ret case repeats EqRet above, while the Vis
+     case repeats EqVis below. *)
+  * punfold Heutt; red in Heutt; cbn in Heutt.
+    rewrite entree_eta. pclearbot. fold_ruttF H.
+    remember (TauF m1) as ot1; revert m1 m2 H Heqot1.
+    induction Heutt as [|m1_bis m1'| |m1_bis ot1' _|t1_bis m1'];
+    intros * Hrutt Heqot1; clear t1'; try discriminate.
+    + inv Heqot1. pclearbot. gfinal; right; pstep; red.
+      apply EqTau. right. now apply (CIH m1).
+    + inv Heqot1. rewrite (entree_eta m1) in Hrutt.
+      desobs m1 Hm1; clear m1 Hm1.
+      { fold_eqitF Heutt. apply eutt_inv_Ret_l in Heutt.
+        rewrite Heutt, tau_euttge. gfinal; right. eapply paco2_mon_bot; eauto. }
+      { apply rutt_inv_Tau_l in Hrutt. eapply IHHeutt; eauto. }
+      { clear IHHeutt. remember (VisF e k) as m1; revert Heqm1.
+        induction Heutt as [| | e1 k1 k1' Hk1k1'| |]; intros; try discriminate.
+        - symmetry in Heqm1; dependent destruction Heqm1.
+          rewrite tau_euttge, (entree_eta m2).
+          punfold Hrutt; red in Hrutt; cbn in Hrutt.
+          remember (VisF e1 k1) as m1; revert Heqm1.
+          induction Hrutt; intros; try discriminate.
+          * dependent destruction Heqm1.
+            gfinal; right. pstep; red; cbn.
+            apply EqVis; auto. intros v1 v2 HAns. specialize (H0 v1 v2 HAns).
+            hnf in H0; hnf. pclearbot; right. apply (CIH (k1 v1)); auto.
+            apply Hk1k1'.
+          * idtac. rewrite tau_euttge, (entree_eta t2). now apply IHHrutt.
+        - idtac. rewrite tau_euttge, entree_eta; now apply IHHeutt. }
+    + inv Heqot1. gfinal; right. pstep; red. apply EqTau. right.
+      fold_eqitF Heutt. rewrite tau_euttge in Heutt. now apply (CIH m1).
+
+  (* EqVis: Similar to EqRet, but we don't have t1' ≳ Vis e1 k1 because the
+     continuations are "only" ≈. The up-to-eutt principle that enforces Vis
+     steps could work, but we don't have it for rutt. Instead we peel the Tau
+     layers off t1' with a manual induction. *)
+  * rewrite entree_eta. gfinal; right; pstep.
+    rename H0 into HAns. punfold Heutt; red in Heutt; cbn in Heutt.
+    remember (VisF e1 k1) as m1; revert Heqm1.
+    induction Heutt; intros; try discriminate.
+    + dependent destruction Heqm1.
+      apply EqVis; auto. intros a b HAns'. specialize (HAns a b HAns').
+      hnf in HAns; hnf. pclearbot; right. apply (CIH (k1 a)); auto. apply REL.
+    + now apply EqTauL, IHHeutt.
+
+  (* EqTauL: We get a very strong IHHrutt at the ruttF level, which we can
+     apply immediately; then handle the added Tau in ≈, which is trivial. *)
+  * apply IHHrutt. rewrite <- entree_eta. now rewrite <- tau_eutt.
+
+  (* EqTauR: Adding a Tau on the side of t2 changes absolutely nothing to the
+     way we rewrite t1, so we can follow down and recurse. *)
+  * rewrite tau_euttge. rewrite (entree_eta t0). now apply IHHrutt.
+Qed.
+
+#[global] Instance rutt_Proper_R3 {E1 E2 R1 R2}
+  `{enc1 : EncodedType E1} `{enc2 : EncodedType E2}:
+  Proper (eq_rel         (* REv *)
+      ==> PostRelEq        (* RAns *)
+      ==> @eq_rel R1 R2  (* RR *)
+      ==> eutt eq        (* t1 *)
+      ==> eutt eq        (* t2 *)
+      ==> iff) (@rutt E1 E2 _ _ R1 R2).
+Proof.
+  intros REv REv2 HREv RAns RAns2 HRAns RR RR2 HRR t1 t1' Ht1 t2 t2' Ht2.
+  rewrite <- HREv, <- HRAns, <- HRR; clear HREv REv2 HRAns RAns2 HRR RR2.
+  split; intros Hrutt.
+  - eapply rutt_cong_eutt; eauto.
+    rewrite rutt_flip in *. eapply rutt_cong_eutt; eauto.
+  - symmetry in Ht1, Ht2.
+    eapply rutt_cong_eutt; eauto.
+    rewrite rutt_flip in *. eapply rutt_cong_eutt; eauto.
+Qed.
+
+(* Bind closure and bind lemmas. *)
+Ltac auto_ctrans :=
+  intros; repeat (match goal with [H: rcompose _ _ _ _ |- _] => destruct H end); subst; eauto.
+Ltac auto_ctrans_eq := try instantiate (1:=eq); auto_ctrans.
+Section RuttBind.
+Context {E1 E2 : Type} `{enc1 : EncodedType E1} `{enc2 : EncodedType E2}.
+Context {R1 R2 : Type}.
+Context (RPre : Rel E1 E2).
+Context (RPost : PostRel E1 E2).
+Context (RR : Rel R1 R2).
+
+Inductive rutt_bind_clo (r : entree E1 R1 -> entree E2 R2 -> Prop) :
+  entree E1 R1 -> entree E2 R2 -> Prop :=
+| rbc_intro_h U1 U2 (RU : U1 -> U2 -> Prop) t1 t2 k1 k2
+      (EQV: rutt RPre RPost RU t1 t2)
+      (REL: forall u1 u2, RU u1 u2 -> r (k1 u1) (k2 u2))
+  : rutt_bind_clo r (EnTree.bind t1 k1) (EnTree.bind t2 k2)
+.
+Hint Constructors rutt_bind_clo: core.
+
+Lemma rutt_clo_bind :
+  rutt_bind_clo <3= gupaco2 (rutt_ RPre RPost RR) (euttge_trans_clo RR).
+Proof.
+  intros rr. gcofix CIH. intros. destruct PR.
+  gclo. econstructor; auto_ctrans_eq.
+  1,2: rewrite unfold_bind; reflexivity.
+  punfold EQV. unfold rutt_ in *.
+  hinduction EQV before CIH; intros; pclearbot; cbn;
+    repeat (change (EnTree.subst ?k ?m) with (EnTree.bind m k)).
+  - gclo. econstructor; auto_ctrans_eq.
+    1,2: reflexivity.
+    eauto with paco.
+  - gstep. econstructor. eauto 7 with paco.
+  - gstep. econstructor; eauto 7 with paco.
+    intros. specialize (H0 a b H1). pclearbot. eauto 7 with paco.
+  - gclo. econstructor; auto_ctrans_eq; cycle -1; eauto; try reflexivity.
+    rewrite tau_euttge.
+    rewrite unfold_bind. reflexivity.
+  - gclo. econstructor; auto_ctrans_eq; cycle -1; eauto; try reflexivity.
+    rewrite tau_euttge. rewrite unfold_bind. reflexivity.
+Qed.
+
+End RuttBind.
+
+Lemma rutt_bind {E1 E2 R1 R2 T1 T2} `{EncodedType E1} `{EncodedType E2}
+      (RPre : Rel E1 E2)
+      (RPost : PostRel E1 E2)
+      (RR: R1 -> R2 -> Prop) (RT: T1 -> T2 -> Prop) t1 t2 k1 k2:
+    rutt RPre RPost RR t1 t2 ->
+    (forall r1 r2,
+      RR r1 r2 ->
+      rutt RPre RPost RT (k1 r1) (k2 r2)) ->
+    rutt RPre RPost RT (EnTree.bind t1 k1) (EnTree.bind t2 k2).
+Proof.
+  intros. ginit.
+  (* For some reason [guclo] fails, apparently trying to infer the type in a
+     context with less information? *)
+  eapply gpaco2_uclo; [|eapply rutt_clo_bind|]; eauto with paco.
+  econstructor; eauto. intros; subst. gfinal. right. apply H2. eauto.
+Qed.
